theories/heap_lang/proofmode.v
@@ -511,7 +511,7 @@ Tactic Notation "wp_cas_suc" :=
     |try congruence
     |try fast_done (* vals_cas_compare_safe *)
     |simpl; try wp_value_head]
-  | |- envs_entails _ (twp ?E ?e ?Q) =>
+  | |- envs_entails _ (twp ?s ?E ?e ?Q) =>
     first
       [reshape_expr e ltac:(fun K e' => eapply (tac_twp_cas_suc _ _ _ _ _ K))
       |fail 1 "wp_cas_suc: cannot find 'CAS' in" e];
